src/tls/Hashing.CRF.fst
@@ -2,13 +2,8 @@
 module Hashing.CRF
 
 open Mem
-include Hashing
+open Hashing
 open FStar.Bytes
-
-//2018.04.24 SZ: to be moved elsewhere, set to false for real extraction
-inline_for_extraction
-val crf: alg -> Tot bool
-let crf _ = false
 
 (* Depending on a single, global idealization function, we keep a global
     inverse table for all (finalized) hash computations, and we use it to
@@ -22,7 +17,7 @@ module MDM = FStar.Monotonic.DependentMap
 // the precise types guarantee that the table stays empty when crf _ = false
 private type range = | Computed: a: alg {crf a} -> t: tag a -> range
 private type domain (r:range) =
-  b:bytes {let Computed a t = r in length b <= max_input_length a /\ h a b = t}
+  b:bytes {let Computed a t = r in length b <= max_input_length a /\ h_ a b = t}
 
 private let inv (f:MDM.partial_dependent_map range domain) = True // a bit overkill?
 private let table : MDM.t tls_tables_region range domain inv = MDM.alloc()
@@ -32,21 +27,18 @@ private let table : MDM.t tls_tables_region range domain inv = MDM.alloc()
 // (not sure how to manage that table)
 
 //val hashed: a:alg -> b:bytes -> Type
-abstract type hashed (a:alg) (b:hashable a) =
+type hashed (a:alg) (b:hashable a) =
   crf a ==> (
-    let t = h a b in
+    let t = h_ a b in
     let b: domain (Computed a t) = b in
     witnessed (MDM.contains table (Computed a t) b))
 
-val crf_injective (a:alg) (b0 b1:hashable a): ST unit  // should be STTot
-  (requires fun h0 -> hashed a b0 /\ hashed a b1)
-  (ensures fun t0 _ t1 -> t0 == t1 /\ (crf a /\ h a b0 =  h a b1 ==> b0 = b1))
 let crf_injective a b0 b1 =
   if crf a then (
     recall table;
     let f = !table in
-    testify(MDM.contains table (Computed a (h a b0)) b0);
-    testify(MDM.contains table (Computed a (h a b1)) b1)
+    testify(MDM.contains table (Computed a (h_ a b0)) b0);
+    testify(MDM.contains table (Computed a (h_ a b1)) b1)
   )
 
 /// We use [stop] to model the exclusion of "bad" events, in this case
@@ -58,14 +50,6 @@ private val stop: s:string -> ST 'a
   (ensures (fun h0 r h1 -> False))
 let rec stop (s:string) = stop s
 
-
-val finalize: #a:alg -> v:accv a -> ST (tag a)
-  (requires (fun h0 -> True))
-  (ensures (fun h0 t h1 ->
-    let b = content v in
-    //18-01-03 TODO modifies (Set.as_set [TLSConstants.tls_tables_region]) h0 h1 /\
-    t = h a b /\ hashed a b
-  ))
 
 #set-options "--admit_smt_queries true" //18-02-26 was verified with MonotonicMap
 let finalize #a v =
